deps/poulet4/lib/LightTyping/LvalueTyping.v
@@ -1,0 +1,48 @@
+Require Export Poulet4.LightTyping.ValueTyping Coq.ZArith.BinInt.
+
+(** L-value typing. *)
+
+Section Tags.
+  Context {tags_t:Type}.
+  Notation typ := (@P4Type tags_t).
+  Notation lvalue := (@ValueLvalue tags_t).
+  
+  Definition typ_of_lv '(MkValueLvalue _ t : lvalue) : typ := t.
+
+  (** Typing analogue to [Semantics.loc_to_sval]. *)
+  Definition typ_of_loc_var
+             (l: Locator) (g: PathMap.t typ) : option typ :=
+    match l with
+    | LInstance p => PathMap.get p g
+    | LGlobal   _ => None
+    end.
+End Tags.
+
+Reserved Notation "x '⊢ₗ' lv" (at level 80, no associativity).
+
+Inductive lval_typ
+          {tags_t : Type}
+          (Δ : list String.string) (Γ : PathMap.t (@P4Type tags_t))
+  : @ValueLvalue tags_t -> Prop :=
+| typ_left_name x l τ :
+    typ_of_loc_var l Γ = Some τ ->
+    Δ ⊢ok τ ->
+    (Δ,Γ) ⊢ₗ MkValueLvalue (ValLeftName x l) τ
+| typ_left_member lv x τ τs :
+    AList.get (P4String.clear_AList_tags τs) x = Some τ ->
+    member_type τs (typ_of_lv lv) ->
+    Δ ⊢ok τ ->
+    (Δ,Γ) ⊢ₗ lv ->
+    (Δ,Γ) ⊢ₗ MkValueLvalue (ValLeftMember lv x) τ
+| typ_left_bit_access lv hi lo w :
+    (lo <= hi < w)%N ->
+    typ_of_lv lv = TypBit w ->
+    (Δ,Γ) ⊢ₗ lv ->
+    (Δ,Γ) ⊢ₗ MkValueLvalue (ValLeftBitAccess lv hi lo) (TypBit (hi - lo + 1)%N)
+| typ_left_array_access lv (z : Z) τ n :
+    (0 <= z)%Z ->
+    typ_of_lv lv = TypArray τ n ->
+    (Δ,Γ) ⊢ₗ lv ->
+    (Δ,Γ) ⊢ₗ MkValueLvalue (ValLeftArrayAccess lv z) τ
+where "x '⊢ₗ' lv"
+        := (lval_typ (fst x) (snd x) lv) : type_scope.
